added memory-relevent features---global variables, struct/array, load/store/GEP/alloca, extract/insertvalue. Static/dynamic rules about new features are admitted.
git-svn-id: https://webdav.seas.upenn.edu/svn/sol/vol@2479 eef5ea85-cc2e-0410-bd84-0fae1f012da8

src/ssa/llvm_op/ssa_interpreter.v
@@ -169,8 +169,9 @@ Definition switchToNewBasicBlock (Dest:block) (PrevBB:block) (Values:Mem): (bloc
 Definition getOperandValue (v:value) (Values:Mem) : option GenericValue := 
 match v with
 | value_id id => Values id
-| value_constant (const_val n) => Some (GenericValue_int n)
+| value_constant (const_int n) => Some (GenericValue_int n)
 | value_constant const_undef => Some (GenericValue_int 0)
+| _ => None
 end.
 
 Fixpoint params2OpGenericValues (lp:list_param) (Values:Mem) : list (option GenericValue):=
